Common/COption.v
@@ -99,27 +99,132 @@ Global Instance eq_some_unfold_bind_guard `{Decision P} {A} (oa : option A) a Q:
 Proof. tcclean. case_guard; rewrite eq_some_unfold; naive_solver. Qed.
 
 
-(** * CDestrEqSome *)
+(** * EqNoneUnfold *)
 
-(** To enable unfolding of some equality, use this *)
-Class CDestrEqSome := cdestr_eq_some {}.
+Class EqNoneUnfold {A} (oa : option A) (P : Prop) :=
+  {eq_none_unfold : oa = None ↔ P}.
+Global Hint Mode EqNoneUnfold + + - : typeclass_instances.
 
-#[export] Instance cdestr_eq_some_dir `{CDestrEqSome} `{EqSomeUnfold T oa a P}
-  `{∀ x, Unconvertible (option T) oa (Some x)}
-  `{Unconvertible Prop (oa = Some a) P} :
-  CDestrSimpl (oa = Some a) P :=
-  cdestr_simpl (@eq_some_unfold T oa a P _).
+Global Instance eq_none_unfold_default {A} (oa : option A):
+  EqNoneUnfold oa (oa = None) | 1000.
+Proof. by tcclean. Qed.
 
-#[export] Instance cdestr_eq_some_rev `{CDestrEqSome} `{EqSomeUnfold T oa a P}
-  `{∀ x, Unconvertible (option T) oa (Some x)}
-  `{Unconvertible Prop (oa = Some a) P} :
-    CDestrSimpl (Some a = oa) P.
-Proof. sfirstorder. Qed.
+Global Instance eq_none_unfold_Some {A} (a : A):
+  EqNoneUnfold (Some a) False.
+Proof. by tcclean. Qed.
 
-(** * Hint database for options *)
-Hint Extern 5 (_ = Some _) => progress (apply eq_some_unfold) : option.
-Hint Extern 5 (Some _ = _) => progress (apply eq_some_unfold) : option.
+Global Instance eq_none_unfold_None {A}:
+  EqNoneUnfold (@None A) True.
+Proof. by tcclean. Qed.
+
+Global Instance eq_none_unfold_mret {A} (a : A):
+  EqNoneUnfold (mret a) False.
+Proof. tcclean. unfold mret. unfold option_ret. done. Qed.
+
+Global Instance eq_none_unfold_mfail {A} (a : A):
+  @EqNoneUnfold A mfail True.
+Proof. tcclean. unfold mfail. unfold option_mfail. done. Qed.
+
+Global Instance eq_none_unfold_fmap {A B} (f : A → B) ma P:
+  EqNoneUnfold ma P →
+  EqNoneUnfold (f <$> ma) P.
+Proof. tcclean. apply fmap_None. Qed.
 
 Global Instance incomptible_None_Some {A} (a : option A) (b : A) :
   Incompatible (a = None) (a = Some b).
 Proof. tcclean. cdestruct a |- **. Qed.
+
+
+(* TODO figure out how to do the bind case in a nice way *)
+#[local] Instance eq_none_unfold_bind {A B} (f : A → option B) ma P Q:
+  (∀ a, EqSomeUnfold ma a (P a)) →
+  (∀ a, EqNoneUnfold (f a) (Q a)) →
+  EqNoneUnfold (ma ≫= f) (∀ a, P a → Q a) | 20.
+Proof.
+  tcclean. rewrite bind_None. cdestruct |- *** # CDestrSplitGoal.
+  + congruence.
+  + classical_right.
+    rewrite not_eq_None_Some in H2.
+    unfold is_Some in H2.
+    cdestruct H2.
+    naive_solver.
+Qed.
+
+Global Instance eq_none_unfold_bind_guard `{Decision P} {A} (oa : option A) Q:
+  EqNoneUnfold oa Q →
+  EqNoneUnfold (guard P;; oa) (¬ P ∨ Q) | 10.
+Proof. tcclean. case_guard; rewrite eq_none_unfold; naive_solver. Qed.
+
+
+(** * CDestrEqSome *)
+
+(** To enable unfolding of option equality, use this *)
+Class CDestrEqOpt := cdestr_eq_opt {}.
+
+Tactic Notation "eunify" open_constr(x) open_constr(y) "with" ident(h) :=
+  unify x y with h.
+
+
+Class TCNotSome {T} (o : option T) := {}.
+Global Hint Extern 1 (TCNotSome ?o) =>
+         (assert_fails (eunify o (Some _) with typeclass_instances); constructor)
+         : typeclass_instances.
+
+Notation TCNotNone T o := (Unconvertible (option T) None o).
+
+#[export] Instance cdestr_eq_some_order g `{CDestrEqOpt} {T} a
+  `{TCNotSome T oa}:
+  CDestrSimpl g (Some a = oa) (oa = Some a).
+Proof. tcclean. naive_solver. Qed.
+
+#[export] Instance cdestr_eq_none_order g `{CDestrEqOpt} {T}
+  `{TCNotNone T oa}:
+  CDestrSimpl g (None = oa) (oa = None).
+Proof. tcclean. naive_solver. Qed.
+
+(* TODO, This set of 4 instances is not very efficient, and not general enough *)
+
+#[export] Instance cdestr_eq_some_clean_l g `{CDestrEqOpt} {T} (ob : option T)
+  `{TCNotSome T oa}
+  `{TCFastDone (oa = Some b)} :
+  CDestrSimpl g (oa = ob) (ob = Some b).
+Proof. tcclean. naive_solver. Qed.
+
+#[export] Instance cdestr_eq_some_clean_r g `{CDestrEqOpt} {T} (oa : option T)
+  `{TCNotSome T ob}
+  `{TCFastDone (ob = Some b)} :
+  CDestrSimpl g (oa = ob) (oa = Some b).
+Proof. tcclean. naive_solver. Qed.
+
+#[export] Instance cdestr_eq_nome_clean_l g `{CDestrEqOpt} {T} (ob : option T)
+  `{TCNotNone T oa}
+  `{TCFastDone (oa = None)} :
+  CDestrSimpl g (oa = ob) (ob = None).
+Proof. tcclean. naive_solver. Qed.
+
+#[export] Instance cdestr_eq_none_clean_r g `{CDestrEqOpt} {T} (oa : option T)
+  `{TCNotNone T ob}
+  `{TCFastDone (ob = None)} :
+  CDestrSimpl g (oa = ob) (oa = None).
+Proof. tcclean. naive_solver. Qed.
+
+#[export] Instance cdestr_eq_some_unfold g `{CDestrEqOpt}
+  `{TCNotSome T oa}
+  `{EqSomeUnfold T oa a P}
+  `{Unconvertible Prop (oa = Some a) P} :
+  CDestrSimpl g (oa = Some a) P :=
+  cdestr_simpl g (@eq_some_unfold T oa a P _).
+
+#[export] Instance cdestr_eq_none_unfold g `{CDestrEqOpt}
+  `{TCNotNone T oa}
+  `{EqNoneUnfold T oa P}
+  `{Unconvertible Prop (oa = None) P} :
+  CDestrSimpl g (oa = None) P :=
+  cdestr_simpl g (@eq_none_unfold T oa P _).
+
+
+(** * Hint database for options *)
+Hint Extern 5 (_ = Some _) => progress (apply eq_some_unfold) : option.
+Hint Extern 5 (Some _ = _) => progress (apply eq_some_unfold) : option.
+Hint Extern 5 (_ = None) => progress (apply eq_none_unfold) : option.
+Hint Extern 5 (None = _) => progress (apply eq_none_unfold) : option.
